theories/LogicalRelation.v
@@ -44,6 +44,7 @@ Set Implicit Arguments.
 
 Module LR.
 
+  Import World.notations.
   Import (hints) Tri.
   Import Pred.
   Import Pred.notations.
@@ -63,11 +64,11 @@ Module LR.
   Definition RBox Θ {transΘ : Trans Θ} {instΘ : forall w, Inst (Θ w) (Assignment w)}
      {A} (R : RELATION Θ A) : RELATION Θ (Box Θ A) :=
     fun w0 w1 θ01 ba0 ba1 =>
-       ∀ₚ w2 ∶ Const World,
-       ∀ₚ w3 ∶ Const World,
-       ∀ₚ θ02 ∶ Const (Θ w0 w2),
-       ∀ₚ θ13 ∶ Const (Θ w1 w3),
-       ∀ₚ θ23 ∶ Const (Θ w2 w3),
+       ∀ₚ w2 ∶ World,
+       ∀ₚ w3 ∶ World,
+       ∀ₚ θ02 ∶ Θ w0 w2,
+       ∀ₚ θ13 ∶ Θ w1 w3,
+       ∀ₚ θ23 ∶ Θ w2 w3,
          Acc.wlp θ13
            (θ01 ⊙ θ13 =ₚ θ02 ⊙ θ23 ->ₚ
             R w2 w3 θ23 (ba0 w2 θ02) (ba1 w3 θ13)).
@@ -88,7 +89,7 @@ Module LR.
     fun w0 w1 θ01 da0 da1 =>
       match da0 , da1 with
       | (w2; (θ02,a2)) , (w3; (θ13,a3)) =>
-          ∃ₚ θ23 ∶ Const (Θ w2 w3),
+          ∃ₚ θ23 ∶ Θ w2 w3,
           Acc.wp θ13
             ((θ01 ⊙ θ13) =ₚ (θ02 ⊙ θ23) /\ₚ
              R w2 w3 θ23 a2 a3)
@@ -96,8 +97,8 @@ Module LR.
 
   Definition RImpl {Θ A B} (RA : RELATION Θ A) (RB : RELATION Θ B) : RELATION Θ (Impl A B) :=
     fun w0 w1 θ01 f0 f1 =>
-      (∀ₚ a0 ∶ Const (A w0),
-       ∀ₚ a1 ∶ Const (A w1),
+      (∀ₚ a0 ∶ A w0,
+       ∀ₚ a1 ∶ A w1,
          RA w0 w1 θ01 a0 a1 ->ₚ
          RB w0 w1 θ01 (f0 a0) (f1 a1))%P.
 
